Makefile
@@ -1,12 +1,16 @@
 default: clean while.exe
 
 clean:
-	rm -f *.dll *.mdb *.exe while.cs
+	rm -f *.dll *.mdb *.exe while.cs whileref.cs
 
 while.exe: while.dfy ReadFileNative.cs
 	dafny while.dfy ReadFileNative.cs
 
-test: while.exe
+whileref.exe: whileref.dfy ReadFileNative.cs
+	dafny whileref.dfy ReadFileNative.cs
+
+test: while.exe whileref.exe
 	mono while.exe ex1.whl
 	mono while.exe ex2.whl
 	mono while.exe ex3.whl
+	mono whileref.exe ex4.whl
